Finish adding permissions, begin to fix injections
Add compartment principals to remaining memory operations, fix and prove
standard lemmas. After that, extend memory injections with ownership
information and start to amend their metatheory.

Standard injections are done, working through extensions.

common/Memory.v
@@ -485,18 +485,20 @@ Next Obligation.
   eapply nextblock_compartments; eauto.
 Qed.
 
-Definition free (m: mem) (b: block) (lo hi: Z): option mem :=
-  if range_perm_dec m b lo hi Cur Freeable
+Definition free (m: mem) (b: block) (lo hi: Z) (cp: compartment): option mem :=
+  if range_perm_dec m b lo hi Cur Freeable &&
+     own_block_dec m b cp
   then Some(unchecked_free m b lo hi)
   else None.
 
-Fixpoint free_list (m: mem) (l: list (block * Z * Z)) {struct l}: option mem :=
+(* RB: NOTE: Add compartments to each item in the list? *)
+Fixpoint free_list (m: mem) (l: list (block * Z * Z)) (cp: compartment) {struct l}: option mem :=
   match l with
   | nil => Some m
   | (b, lo, hi) :: l' =>
-      match free m b lo hi with
+      match free m b lo hi cp with
       | None => None
-      | Some m' => free_list m' l'
+      | Some m' => free_list m' l' cp
       end
   end.
 
@@ -678,19 +680,24 @@ Next Obligation.
   now apply nextblock_compartments.
 Qed.
 
-(** [drop_perm m b lo hi p] sets the max permissions of the byte range
-    [(b, lo) ... (b, hi - 1)] to [p].  These bytes must have current permissions
-    [Freeable] in the initial memory state [m].
+(** [drop_perm m b lo hi p cp] sets the max permissions of the byte range
+    [(b, lo) ... (b, hi - 1)] to [p] performed from compartment [cp].  These
+    bytes must have current permissions [Freeable] in the initial memory state
+    [m].
     Returns updated memory state, or [None] if insufficient permissions. *)
 
-Program Definition drop_perm (m: mem) (b: block) (lo hi: Z) (p: permission): option mem :=
+(* RB: NOTE: Ownership permissions added by nested conditionals to work around
+   funny [Program Definition] misbehavior in the second [Obligation]. *)
+Program Definition drop_perm (m: mem) (b: block) (lo hi: Z) (p: permission) (cp: compartment): option mem :=
   if range_perm_dec m b lo hi Cur Freeable then
-    Some (mkmem m.(mem_contents)
-                (PMap.set b
-                        (fun ofs k => if zle lo ofs && zlt ofs hi then Some p else m.(mem_access)#b ofs k)
-                        m.(mem_access))
-                m.(mem_compartments)
-                m.(nextblock) _ _ _ _)
+    if own_block_dec m b cp then
+      Some (mkmem m.(mem_contents)
+                      (PMap.set b
+                                (fun ofs k => if zle lo ofs && zlt ofs hi then Some p else m.(mem_access)#b ofs k)
+                                m.(mem_access))
+                      m.(mem_compartments)
+                          m.(nextblock) _ _ _ _)
+    else None
   else None.
 Next Obligation.
   repeat rewrite PMap.gsspec. destruct (peq b0 b). subst b0.
@@ -698,11 +705,11 @@ Next Obligation.
   apply access_max.
 Qed.
 Next Obligation.
-  specialize (nextblock_noaccess m b0 ofs k H0). intros.
+  specialize (nextblock_noaccess m b0 ofs k H1). intros.
   rewrite PMap.gsspec. destruct (peq b0 b). subst b0.
   destruct (zle lo ofs). destruct (zlt ofs hi).
   assert (perm m b ofs k Freeable). apply perm_cur. apply H; auto.
-  unfold perm in H2. rewrite H1 in H2. contradiction.
+  unfold perm in H3. rewrite H2 in H3. contradiction.
   auto. auto. auto.
 Qed.
 Next Obligation.
@@ -1985,9 +1992,9 @@ Proof.
 Qed.
 
 Theorem unowned_fresh_block:
-  ~own_block m1 b c.
+  forall c', ~own_block m1 b c'.
 Proof.
-  unfold own_block. intro Hcontra.
+  unfold own_block. intros c' Hcontra.
   unfold alloc in ALLOC. destruct m1. inv ALLOC. simpl in *.
   rewrite (proj1 (nextblock_compartments0 b)) in Hcontra.
   - inversion Hcontra.
@@ -2240,11 +2247,12 @@ Local Hint Resolve valid_access_alloc_other valid_access_alloc_same: mem.
 (** ** Properties related to [free]. *)
 
 Theorem range_perm_free:
-  forall m1 b lo hi,
+  forall m1 b lo hi cp,
   range_perm m1 b lo hi Cur Freeable ->
-  { m2: mem | free m1 b lo hi = Some m2 }.
+  own_block m1 b cp ->
+  { m2: mem | free m1 b lo hi cp = Some m2 }.
 Proof.
-  intros; unfold free. rewrite pred_dec_true; auto. econstructor; eauto.
+  intros; unfold free. econstructor. setoid_rewrite pred_dec_true; auto. simpl. eauto.
 Defined.
 
 Section FREE.
@@ -2252,21 +2260,26 @@ Section FREE.
 Variable m1: mem.
 Variable bf: block.
 Variables lo hi: Z.
+Variable cp: compartment.
 Variable m2: mem.
-Hypothesis FREE: free m1 bf lo hi = Some m2.
+Hypothesis FREE: free m1 bf lo hi cp = Some m2.
 
 Theorem free_range_perm:
   range_perm m1 bf lo hi Cur Freeable.
 Proof.
   unfold free in FREE. destruct (range_perm_dec m1 bf lo hi Cur Freeable); auto.
+  destruct (own_block_dec m1 bf cp); simpl in FREE;
   congruence.
 Qed.
 
 Lemma free_result:
   m2 = unchecked_free m1 bf lo hi.
 Proof.
-  unfold free in FREE. destruct (range_perm_dec m1 bf lo hi Cur Freeable).
-  congruence. congruence.
+  unfold free in FREE.
+  destruct (range_perm_dec m1 bf lo hi Cur Freeable);
+  destruct (own_block_dec m1 bf cp);
+  simpl in FREE;
+  congruence.
 Qed.
 
 Theorem nextblock_free:
@@ -2334,21 +2347,63 @@ Proof.
   destruct (zlt ofs hi); simpl; auto.
 Qed.
 
-Theorem valid_access_free_1:
-  forall chunk b ofs p,
-  valid_access m1 chunk b ofs p ->
-  b <> bf \/ lo >= hi \/ ofs + size_chunk chunk <= lo \/ hi <= ofs ->
-  valid_access m2 chunk b ofs p.
+Lemma free_own_block_1 : own_block m1 bf cp.
 Proof.
-  intros. inv H. constructor; auto with mem.
+  unfold free in FREE.
+  destruct (range_perm_dec m1 bf lo hi Cur Freeable);
+    destruct (own_block_dec m1 bf cp);
+    simpl in FREE;
+    congruence.
+Qed.
+
+Lemma free_own_block_2 : own_block m2 bf cp.
+Proof.
+  unfold free in FREE.
+  destruct (range_perm_dec m1 bf lo hi Cur Freeable);
+    destruct (own_block_dec m1 bf cp);
+    inv FREE.
+  assumption.
+Qed.
+
+Lemma free_own_block_inj_1 :
+  forall b cp', own_block m1 b cp' -> own_block m2 b cp'.
+Proof.
+  unfold own_block.
+  intros b cp' Hown.
+  unfold free in FREE.
+  destruct (range_perm_dec m1 bf lo hi Cur Freeable); [| simpl in FREE; congruence].
+  destruct (own_block_dec m1 bf cp); [| simpl in FREE; congruence].
+  inv FREE. rewrite <- Hown. reflexivity.
+Qed.
+
+Lemma free_own_block_inj_2 :
+  forall b cp', own_block m2 b cp' -> own_block m1 b cp'.
+Proof.
+  unfold own_block.
+  intros b cp' Hown.
+  unfold free in FREE.
+  destruct (range_perm_dec m1 bf lo hi Cur Freeable); [| simpl in FREE; congruence].
+  destruct (own_block_dec m1 bf cp); [| simpl in FREE; congruence].
+  inv FREE. rewrite <- Hown. reflexivity.
+Qed.
+
+Theorem valid_access_free_1:
+  forall chunk b ofs p cp',
+  valid_access m1 chunk b ofs p cp' ->
+  b <> bf \/ lo >= hi \/ ofs + size_chunk chunk <= lo \/ hi <= ofs ->
+  valid_access m2 chunk b ofs p cp'.
+Proof.
+  intros. inv H. destruct H2 as [H2 H3]. constructor; auto with mem.
   red; intros. eapply perm_free_1; eauto.
   destruct (zlt lo hi). intuition. right. omega.
+  split; auto.
+  apply free_own_block_inj_1; auto.
 Qed.
 
 Theorem valid_access_free_2:
-  forall chunk ofs p,
+  forall chunk ofs p cp',
   lo < hi -> ofs + size_chunk chunk > lo -> ofs < hi ->
-  ~(valid_access m2 chunk bf ofs p).
+  ~(valid_access m2 chunk bf ofs p cp').
 Proof.
   intros; red; intros. inv H2.
   generalize (size_chunk_pos chunk); intros.
@@ -2360,9 +2415,9 @@ Proof.
 Qed.
 
 Theorem valid_access_free_inv_1:
-  forall chunk b ofs p,
-  valid_access m2 chunk b ofs p ->
-  valid_access m1 chunk b ofs p.
+  forall chunk b ofs p cp',
+  valid_access m2 chunk b ofs p cp' ->
+  valid_access m1 chunk b ofs p cp'.
 Proof.
   intros. destruct H. split; auto.
   red; intros. generalize (H ofs0 H1).
@@ -2371,27 +2426,30 @@ Proof.
   destruct (zle lo ofs0); simpl.
   destruct (zlt ofs0 hi); simpl.
   tauto. auto. auto. auto.
+  split.
+  apply free_own_block_inj_2; easy.
+  easy.
 Qed.
 
 Theorem valid_access_free_inv_2:
-  forall chunk ofs p,
-  valid_access m2 chunk bf ofs p ->
+  forall chunk ofs p cp',
+  valid_access m2 chunk bf ofs p cp' ->
   lo >= hi \/ ofs + size_chunk chunk <= lo \/ hi <= ofs.
 Proof.
   intros.
   destruct (zlt lo hi); auto.
   destruct (zle (ofs + size_chunk chunk) lo); auto.
   destruct (zle hi ofs); auto.
-  elim (valid_access_free_2 chunk ofs p); auto. omega.
+  elim (valid_access_free_2 chunk ofs p cp'); auto. omega.
 Qed.
 
 Theorem load_free:
-  forall chunk b ofs,
+  forall chunk b ofs cp',
   b <> bf \/ lo >= hi \/ ofs + size_chunk chunk <= lo \/ hi <= ofs ->
-  load chunk m2 b ofs = load chunk m1 b ofs.
+  load chunk m2 b ofs cp' = load chunk m1 b ofs cp'.
 Proof.
   intros. unfold load.
-  destruct (valid_access_dec m2 chunk b ofs Readable).
+  destruct (valid_access_dec m2 chunk b ofs Readable cp').
   rewrite pred_dec_true.
   rewrite free_result; auto.
   eapply valid_access_free_inv_1; eauto.
@@ -2400,37 +2458,46 @@ Proof.
 Qed.
 
 Theorem load_free_2:
-  forall chunk b ofs v,
-  load chunk m2 b ofs = Some v -> load chunk m1 b ofs = Some v.
+  forall chunk b ofs v cp',
+  load chunk m2 b ofs cp' = Some v -> load chunk m1 b ofs cp' = Some v.
 Proof.
   intros. unfold load. rewrite pred_dec_true.
-  rewrite (load_result _ _ _ _ _ H). rewrite free_result; auto.
+  rewrite (load_result _ _ _ _ _ _ H). rewrite free_result; auto.
   apply valid_access_free_inv_1. eauto with mem.
 Qed.
 
 Theorem loadbytes_free:
-  forall b ofs n,
+  forall b ofs n cp',
   b <> bf \/ lo >= hi \/ ofs + n <= lo \/ hi <= ofs ->
-  loadbytes m2 b ofs n = loadbytes m1 b ofs n.
+  loadbytes m2 b ofs n cp' = loadbytes m1 b ofs n cp'.
 Proof.
   intros. unfold loadbytes.
   destruct (range_perm_dec m2 b ofs (ofs + n) Cur Readable).
-  rewrite pred_dec_true.
+- destruct (own_block_dec m2 b cp').
++ simpl.
+  setoid_rewrite pred_dec_true.
   rewrite free_result; auto.
   red; intros. eapply perm_free_3; eauto.
-  rewrite pred_dec_false; auto.
+  apply free_own_block_inj_2; assumption.
++ simpl. setoid_rewrite pred_dec_false at 2.
+  rewrite andb_comm. reflexivity.
+  intro Hcontra. apply n0. apply free_own_block_inj_1; assumption.
+- simpl. setoid_rewrite pred_dec_false at 1; auto.
   red; intros. elim n0; red; intros.
   eapply perm_free_1; eauto. destruct H; auto. right; omega.
 Qed.
 
 Theorem loadbytes_free_2:
-  forall b ofs n bytes,
-  loadbytes m2 b ofs n = Some bytes -> loadbytes m1 b ofs n = Some bytes.
+  forall b ofs n cp' bytes,
+  loadbytes m2 b ofs n cp' = Some bytes -> loadbytes m1 b ofs n cp' = Some bytes.
 Proof.
   intros. unfold loadbytes in *.
-  destruct (range_perm_dec m2 b ofs (ofs + n) Cur Readable); inv H.
-  rewrite pred_dec_true. rewrite free_result; auto.
+  destruct (range_perm_dec m2 b ofs (ofs + n) Cur Readable);
+  destruct (own_block_dec m2 b cp');
+  inv H.
+  setoid_rewrite pred_dec_true. rewrite free_result; auto.
   red; intros. apply perm_free_3; auto.
+  apply free_own_block_inj_2; assumption.
 Qed.
 
 End FREE.
@@ -2442,18 +2509,24 @@ Local Hint Resolve valid_block_free_1 valid_block_free_2
 (** ** Properties related to [drop_perm] *)
 
 Theorem range_perm_drop_1:
-  forall m b lo hi p m', drop_perm m b lo hi p = Some m' -> range_perm m b lo hi Cur Freeable.
+  forall m b lo hi p m' cp, drop_perm m b lo hi p cp = Some m' -> range_perm m b lo hi Cur Freeable.
 Proof.
   unfold drop_perm; intros.
   destruct (range_perm_dec m b lo hi Cur Freeable). auto. discriminate.
 Qed.
 
 Theorem range_perm_drop_2:
-  forall m b lo hi p,
-  range_perm m b lo hi Cur Freeable -> {m' | drop_perm m b lo hi p = Some m' }.
+  forall m b lo hi cp p,
+  range_perm m b lo hi Cur Freeable ->
+  own_block m b cp ->
+  {m' | drop_perm m b lo hi p cp = Some m' }.
 Proof.
   unfold drop_perm; intros.
-  destruct (range_perm_dec m b lo hi Cur Freeable). econstructor. eauto. contradiction.
+  destruct (range_perm_dec m b lo hi Cur Freeable).
+- destruct (own_block_dec m b cp).
++ econstructor. eauto.
++ contradiction.
+- contradiction.
 Defined.
 
 Section DROP.
@@ -2462,13 +2535,17 @@ Variable m: mem.
 Variable b: block.
 Variable lo hi: Z.
 Variable p: permission.
+Variable cp: compartment.
 Variable m': mem.
-Hypothesis DROP: drop_perm m b lo hi p = Some m'.
+Hypothesis DROP: drop_perm m b lo hi p cp = Some m'.
 
 Theorem nextblock_drop:
   nextblock m' = nextblock m.
 Proof.
-  unfold drop_perm in DROP. destruct (range_perm_dec m b lo hi Cur Freeable); inv DROP; auto.
+  unfold drop_perm in DROP.
+  destruct (range_perm_dec m b lo hi Cur Freeable);
+  destruct (own_block_dec m b cp);
+  inv DROP; auto.
 Qed.
 
 Theorem drop_perm_valid_block_1:
@@ -2487,7 +2564,10 @@ Theorem perm_drop_1:
   forall ofs k, lo <= ofs < hi -> perm m' b ofs k p.
 Proof.
   intros.
-  unfold drop_perm in DROP. destruct (range_perm_dec m b lo hi Cur Freeable); inv DROP.
+  unfold drop_perm in DROP.
+  destruct (range_perm_dec m b lo hi Cur Freeable);
+  destruct (own_block_dec m b cp);
+  inv DROP.
   unfold perm. simpl. rewrite PMap.gss. unfold proj_sumbool.
   rewrite zle_true. rewrite zlt_true. simpl. constructor.
   omega. omega.
@@ -2497,7 +2577,10 @@ Theorem perm_drop_2:
   forall ofs k p', lo <= ofs < hi -> perm m' b ofs k p' -> perm_order p p'.
 Proof.
   intros.
-  unfold drop_perm in DROP. destruct (range_perm_dec m b lo hi Cur Freeable); inv DROP.
+  unfold drop_perm in DROP.
+  destruct (range_perm_dec m b lo hi Cur Freeable);
+  destruct (own_block_dec m b cp);
+  inv DROP.
   revert H0. unfold perm; simpl. rewrite PMap.gss. unfold proj_sumbool.
   rewrite zle_true. rewrite zlt_true. simpl. auto.
   omega. omega.
@@ -2507,7 +2590,10 @@ Theorem perm_drop_3:
   forall b' ofs k p', b' <> b \/ ofs < lo \/ hi <= ofs -> perm m b' ofs k p' -> perm m' b' ofs k p'.
 Proof.
   intros.
-  unfold drop_perm in DROP. destruct (range_perm_dec m b lo hi Cur Freeable); inv DROP.
+  unfold drop_perm in DROP.
+  destruct (range_perm_dec m b lo hi Cur Freeable);
+  destruct (own_block_dec m b cp);
+  inv DROP.
   unfold perm; simpl. rewrite PMap.gsspec. destruct (peq b' b). subst b'.
   unfold proj_sumbool. destruct (zle lo ofs). destruct (zlt ofs hi).
   byContradiction. intuition omega.
@@ -2518,7 +2604,10 @@ Theorem perm_drop_4:
   forall b' ofs k p', perm m' b' ofs k p' -> perm m b' ofs k p'.
 Proof.
   intros.
-  unfold drop_perm in DROP. destruct (range_perm_dec m b lo hi Cur Freeable); inv DROP.
+  unfold drop_perm in DROP.
+  destruct (range_perm_dec m b lo hi Cur Freeable);
+  destruct (own_block_dec m b cp);
+  inv DROP.
   revert H. unfold perm; simpl. rewrite PMap.gsspec. destruct (peq b' b).
   subst b'. unfold proj_sumbool. destruct (zle lo ofs). destruct (zlt ofs hi).
   simpl. intros. apply perm_implies with p. apply perm_implies with Freeable. apply perm_cur.
@@ -2526,10 +2615,49 @@ Proof.
   auto. auto. auto.
 Qed.
 
+Theorem own_block_drop_1:
+  forall b' cp', own_block m b' cp' -> own_block m' b' cp'.
+Proof.
+  unfold own_block. intros b' cp' Hown.
+  unfold drop_perm in DROP.
+  destruct (range_perm_dec m b lo hi Cur Freeable); [| now inversion DROP].
+  destruct (own_block_dec m b cp); [| now inversion DROP].
+  inv DROP. assumption.
+Qed.
+
+Theorem own_block_drop_2:
+  forall b' cp', own_block m' b' cp' -> own_block m b' cp'.
+Proof.
+  unfold own_block. intros b' cp' Hown.
+  unfold drop_perm in DROP.
+  destruct (range_perm_dec m b lo hi Cur Freeable); [| now inversion DROP].
+  destruct (own_block_dec m b cp); [| now inversion DROP].
+  inv DROP. assumption.
+Qed.
+
+Theorem own_block_drop_3:
+  own_block m b cp.
+  unfold drop_perm in DROP.
+  destruct (range_perm_dec m b lo hi Cur Freeable); [| congruence].
+  destruct (own_block_dec m b cp); [| congruence].
+  assumption.
+Qed.
+
+Theorem own_block_drop_4:
+  own_block m' b cp.
+  unfold drop_perm in DROP.
+  destruct (range_perm_dec m b lo hi Cur Freeable); [| congruence].
+  destruct (own_block_dec m b cp); [| congruence].
+  inv DROP. destruct m. unfold own_block in *. simpl in *.
+  assumption.
+Qed.
+
+(* RB: NOTE: Other lemmas in the style of perm_drop_*? *)
+
 Lemma valid_access_drop_1:
-  forall chunk b' ofs p',
+  forall chunk b' ofs p' cp',
   b' <> b \/ ofs + size_chunk chunk <= lo \/ hi <= ofs \/ perm_order p p' ->
-  valid_access m chunk b' ofs p' -> valid_access m' chunk b' ofs p'.
+  valid_access m chunk b' ofs p' cp' -> valid_access m' chunk b' ofs p' cp'.
 Proof.
   intros. destruct H0. split; auto.
   red; intros.
@@ -2539,48 +2667,61 @@ Proof.
   apply perm_implies with p. eapply perm_drop_1; eauto. omega.
   generalize (size_chunk_pos chunk); intros. intuition.
   eapply perm_drop_3; eauto.
+  split. apply own_block_drop_1; easy. easy.
 Qed.
 
 Lemma valid_access_drop_2:
-  forall chunk b' ofs p',
-  valid_access m' chunk b' ofs p' -> valid_access m chunk b' ofs p'.
+  forall chunk b' ofs p' cp',
+  valid_access m' chunk b' ofs p' cp' -> valid_access m chunk b' ofs p' cp'.
 Proof.
   intros. destruct H; split; auto.
   red; intros. eapply perm_drop_4; eauto.
+  split. apply own_block_drop_2; easy. easy.
 Qed.
 
 Theorem load_drop:
-  forall chunk b' ofs,
+  forall chunk b' ofs cp',
   b' <> b \/ ofs + size_chunk chunk <= lo \/ hi <= ofs \/ perm_order p Readable ->
-  load chunk m' b' ofs = load chunk m b' ofs.
+  load chunk m' b' ofs cp' = load chunk m b' ofs cp'.
 Proof.
   intros.
   unfold load.
   destruct (valid_access_dec m chunk b' ofs Readable).
   rewrite pred_dec_true.
-  unfold drop_perm in DROP. destruct (range_perm_dec m b lo hi Cur Freeable); inv DROP. simpl. auto.
+  unfold drop_perm in DROP.
+  destruct (range_perm_dec m b lo hi Cur Freeable);
+  destruct (own_block_dec m b cp);
+  inv DROP. simpl. auto.
   eapply valid_access_drop_1; eauto.
   rewrite pred_dec_false. auto.
   red; intros; elim n. eapply valid_access_drop_2; eauto.
 Qed.
 
 Theorem loadbytes_drop:
-  forall b' ofs n,
+  forall b' ofs n cp',
   b' <> b \/ ofs + n <= lo \/ hi <= ofs \/ perm_order p Readable ->
-  loadbytes m' b' ofs n = loadbytes m b' ofs n.
+  loadbytes m' b' ofs n cp' = loadbytes m b' ofs n cp'.
 Proof.
   intros.
   unfold loadbytes.
   destruct (range_perm_dec m b' ofs (ofs + n) Cur Readable).
-  rewrite pred_dec_true.
-  unfold drop_perm in DROP. destruct (range_perm_dec m b lo hi Cur Freeable); inv DROP. simpl. auto.
-  red; intros.
+- destruct (own_block_dec m b' cp').
++ setoid_rewrite pred_dec_true.
+* unfold drop_perm in DROP.
+  destruct (range_perm_dec m b lo hi Cur Freeable);
+  destruct (own_block_dec m b cp);
+  inv DROP. simpl. auto.
+* red; intros.
   destruct (eq_block b' b). subst b'.
   destruct (zlt ofs0 lo). eapply perm_drop_3; eauto.
   destruct (zle hi ofs0). eapply perm_drop_3; eauto.
   apply perm_implies with p. eapply perm_drop_1; eauto. omega. intuition.
   eapply perm_drop_3; eauto.
-  rewrite pred_dec_false; eauto.
+* apply own_block_drop_1; assumption.
++ setoid_rewrite pred_dec_false at 2.
+* rewrite andb_comm. reflexivity.
+* intro Hcontra. apply n0. apply own_block_drop_2; assumption.
+- setoid_rewrite pred_dec_false at 1; eauto.
   red; intros; elim n0; red; intros.
   eapply perm_drop_4; eauto.
 Qed.
@@ -2604,6 +2745,11 @@ Record mem_inj (f: meminj) (m1 m2: mem) : Prop :=
       f b1 = Some(b2, delta) ->
       perm m1 b1 ofs k p ->
       perm m2 b2 (ofs + delta) k p;
+    mi_own:
+      forall b1 b2 delta cp,
+      f b1 = Some(b2, delta) ->
+      own_block m1 b1 cp ->
+      own_block m2 b2 cp;
     mi_align:
       forall b1 b2 delta chunk ofs p,
       f b1 = Some(b2, delta) ->
@@ -2640,17 +2786,29 @@ Proof.
   eapply perm_inj; eauto. apply H0. omega.
 Qed.
 
+Lemma own_block_inj:
+  forall f m1 m2 b1 cp b2 delta,
+  mem_inj f m1 m2 ->
+  own_block m1 b1 cp ->
+  f b1 = Some(b2, delta) ->
+  own_block m2 b2 cp.
+Proof.
+  intros; red.
+  eapply mi_own; eauto.
+Qed.
+
 Lemma valid_access_inj:
-  forall f m1 m2 b1 b2 delta chunk ofs p,
+  forall f m1 m2 b1 b2 delta chunk ofs p cp,
   mem_inj f m1 m2 ->
   f b1 = Some(b2, delta) ->
-  valid_access m1 chunk b1 ofs p ->
-  valid_access m2 chunk b2 (ofs + delta) p.
+  valid_access m1 chunk b1 ofs p cp ->
+  valid_access m2 chunk b2 (ofs + delta) p cp.
 Proof.
-  intros. destruct H1 as [A B]. constructor.
+  intros. destruct H1 as [A [B C]]. constructor.
   replace (ofs + delta + size_chunk chunk)
      with ((ofs + size_chunk chunk) + delta) by omega.
   eapply range_perm_inj; eauto.
+  split. eapply mi_own; eauto.
   apply Z.divide_add_r; auto. eapply mi_align; eauto with mem.
 Qed.
 
@@ -2677,11 +2835,11 @@ Proof.
 Qed.
 
 Lemma load_inj:
-  forall f m1 m2 chunk b1 ofs b2 delta v1,
+  forall f m1 m2 chunk b1 ofs cp b2 delta v1,
   mem_inj f m1 m2 ->
-  load chunk m1 b1 ofs = Some v1 ->
+  load chunk m1 b1 ofs cp = Some v1 ->
   f b1 = Some (b2, delta) ->
-  exists v2, load chunk m2 b2 (ofs + delta) = Some v2 /\ Val.inject f v1 v2.
+  exists v2, load chunk m2 b2 (ofs + delta) cp = Some v2 /\ Val.inject f v1 v2.
 Proof.
   intros.
   exists (decode_val chunk (getN (size_chunk_nat chunk) (ofs + delta) (m2.(mem_contents)#b2))).
@@ -2693,19 +2851,22 @@ Proof.
 Qed.
 
 Lemma loadbytes_inj:
-  forall f m1 m2 len b1 ofs b2 delta bytes1,
+  forall f m1 m2 len b1 ofs cp b2 delta bytes1,
   mem_inj f m1 m2 ->
-  loadbytes m1 b1 ofs len = Some bytes1 ->
+  loadbytes m1 b1 ofs len cp = Some bytes1 ->
   f b1 = Some (b2, delta) ->
-  exists bytes2, loadbytes m2 b2 (ofs + delta) len = Some bytes2
+  exists bytes2, loadbytes m2 b2 (ofs + delta) len cp = Some bytes2
               /\ list_forall2 (memval_inject f) bytes1 bytes2.
 Proof.
   intros. unfold loadbytes in *.
-  destruct (range_perm_dec m1 b1 ofs (ofs + len) Cur Readable); inv H0.
+  destruct (range_perm_dec m1 b1 ofs (ofs + len) Cur Readable);
+  destruct (own_block_dec m1 b1 cp);
+  inv H0.
   exists (getN (Z.to_nat len) (ofs + delta) (m2.(mem_contents)#b2)).
-  split. apply pred_dec_true.
+  split. setoid_rewrite pred_dec_true. reflexivity.
   replace (ofs + delta + len) with ((ofs + len) + delta) by omega.
   eapply range_perm_inj; eauto with mem.
+  eapply mi_own; eassumption.
   apply getN_inj; auto.
   destruct (zle 0 len). rewrite Z2Nat.id by omega. auto.
   rewrite Z_to_nat_neg by omega. simpl. red; intros; omegaContradiction.
@@ -2740,33 +2901,39 @@ Definition meminj_no_overlap (f: meminj) (m: mem) : Prop :=
   b1' <> b2' \/ ofs1 + delta1 <> ofs2 + delta2.
 
 Lemma store_mapped_inj:
-  forall f chunk m1 b1 ofs v1 n1 m2 b2 delta v2,
+  forall f chunk m1 b1 ofs v1 cp n1 m2 b2 delta v2,
   mem_inj f m1 m2 ->
-  store chunk m1 b1 ofs v1 = Some n1 ->
+  store chunk m1 b1 ofs v1 cp = Some n1 ->
   meminj_no_overlap f m1 ->
   f b1 = Some (b2, delta) ->
   Val.inject f v1 v2 ->
   exists n2,
-    store chunk m2 b2 (ofs + delta) v2 = Some n2
+    store chunk m2 b2 (ofs + delta) v2 cp = Some n2
     /\ mem_inj f n1 n2.
 Proof.
   intros.
-  assert (valid_access m2 chunk b2 (ofs + delta) Writable).
+  assert (valid_access m2 chunk b2 (ofs + delta) Writable cp).
     eapply valid_access_inj; eauto with mem.
-  destruct (valid_access_store _ _ _ _ v2 H4) as [n2 STORE].
+  destruct (valid_access_store _ _ _ _ _ v2 H4) as [n2 STORE].
   exists n2; split. auto.
   constructor.
 (* perm *)
   intros. eapply perm_store_1; [eexact STORE|].
   eapply mi_perm; eauto.
   eapply perm_store_2; eauto.
+(* own *)
+  intros.
+  apply (proj1 (store_own_block_inj _ _ _ _ _ _ _ STORE _ _)).
+  eapply mi_own; try eassumption.
+  apply (proj2 (store_own_block_inj _ _ _ _ _ _ _ H0 _ _)).
+  assumption.
 (* align *)
   intros. eapply mi_align with (ofs := ofs0) (p := p); eauto.
   red; intros; eauto with mem.
 (* mem_contents *)
   intros.
-  rewrite (store_mem_contents _ _ _ _ _ _ H0).
-  rewrite (store_mem_contents _ _ _ _ _ _ STORE).
+  rewrite (store_mem_contents _ _ _ _ _ _ _ H0).
+  rewrite (store_mem_contents _ _ _ _ _ _ _ STORE).
   rewrite ! PMap.gsspec.
   destruct (peq b0 b1). subst b0.
   (* block = b1, block = b2 *)
@@ -2789,43 +2956,52 @@ Proof.
 Qed.
 
 Lemma store_unmapped_inj:
-  forall f chunk m1 b1 ofs v1 n1 m2,
+  forall f chunk m1 b1 ofs v1 cp n1 m2,
   mem_inj f m1 m2 ->
-  store chunk m1 b1 ofs v1 = Some n1 ->
+  store chunk m1 b1 ofs v1 cp = Some n1 ->
   f b1 = None ->
   mem_inj f n1 m2.
 Proof.
   intros. constructor.
 (* perm *)
   intros. eapply mi_perm; eauto with mem.
+(* own *)
+  intros. eapply mi_own; eauto.
+  (* RB: NOTE: Should be solvable by properly extended hint databases. *)
+  apply (proj2 (store_own_block_inj _ _ _ _ _ _ _ H0 _ _)).
+  assumption.
 (* align *)
   intros. eapply mi_align with (ofs := ofs0) (p := p); eauto.
   red; intros; eauto with mem.
 (* mem_contents *)
   intros.
-  rewrite (store_mem_contents _ _ _ _ _ _ H0).
+  rewrite (store_mem_contents _ _ _ _ _ _ _ H0).
   rewrite PMap.gso. eapply mi_memval; eauto with mem.
   congruence.
 Qed.
 
 Lemma store_outside_inj:
-  forall f m1 m2 chunk b ofs v m2',
+  forall f m1 m2 chunk b ofs v cp m2',
   mem_inj f m1 m2 ->
   (forall b' delta ofs',
     f b' = Some(b, delta) ->
     perm m1 b' ofs' Cur Readable ->
     ofs <= ofs' + delta < ofs + size_chunk chunk -> False) ->
-  store chunk m2 b ofs v = Some m2' ->
+  store chunk m2 b ofs v cp = Some m2' ->
   mem_inj f m1 m2'.
 Proof.
   intros. inv H. constructor.
 (* perm *)
   eauto with mem.
+(* own *)
+  intros.
+  (* RB: NOTE: Ditto re: hint databases. *)
+  apply (proj1 (store_own_block_inj _ _ _ _ _ _ _ H1 _ _)); eauto.
 (* access *)
   intros; eapply mi_align0; eauto.
 (* mem_contents *)
   intros.
-  rewrite (store_mem_contents _ _ _ _ _ _ H1).
+  rewrite (store_mem_contents _ _ _ _ _ _ _ H1).
   rewrite PMap.gsspec. destruct (peq b2 b). subst b2.
   rewrite setN_outside. auto.
   rewrite encode_val_length. rewrite <- size_chunk_conv.
@@ -2836,14 +3012,14 @@ Proof.
 Qed.
 
 Lemma storebytes_mapped_inj:
-  forall f m1 b1 ofs bytes1 n1 m2 b2 delta bytes2,
+  forall f m1 b1 ofs bytes1 cp n1 m2 b2 delta bytes2,
   mem_inj f m1 m2 ->
-  storebytes m1 b1 ofs bytes1 = Some n1 ->
+  storebytes m1 b1 ofs bytes1 cp = Some n1 ->
   meminj_no_overlap f m1 ->
   f b1 = Some (b2, delta) ->
   list_forall2 (memval_inject f) bytes1 bytes2 ->
   exists n2,
-    storebytes m2 b2 (ofs + delta) bytes2 = Some n2
+    storebytes m2 b2 (ofs + delta) bytes2 cp = Some n2
     /\ mem_inj f n1 n2.
 Proof.
   intros. inversion H.
@@ -2853,7 +3029,8 @@ Proof.
     eapply range_perm_inj; eauto with mem.
     eapply storebytes_range_perm; eauto.
     rewrite (list_forall2_length H3). omega.
-  destruct (range_perm_storebytes _ _ _ _ H4) as [n2 STORE].
+  destruct (range_perm_storebytes _ _ _ _ cp H4) as [n2 STORE].
+  eapply own_block_inj; try eassumption. eapply storebytes_own_block_1; eassumption.
   exists n2; split. eauto.
   constructor.
 (* perm *)
@@ -2861,14 +3038,19 @@ Proof.
   eapply perm_storebytes_1; [apply STORE |].
   eapply mi_perm0; eauto.
   eapply perm_storebytes_2; eauto.
+(* own *)
+  intros.
+  eapply storebytes_own_block_inj_1; [apply STORE |].
+  eapply mi_own0; eauto.
+  eapply storebytes_own_block_inj_2; eauto.
 (* align *)
   intros. eapply mi_align with (ofs := ofs0) (p := p); eauto.
   red; intros. eapply perm_storebytes_2; eauto.
 (* mem_contents *)
   intros.
   assert (perm m1 b0 ofs0 Cur Readable). eapply perm_storebytes_2; eauto.
-  rewrite (storebytes_mem_contents _ _ _ _ _ H0).
-  rewrite (storebytes_mem_contents _ _ _ _ _ STORE).
+  rewrite (storebytes_mem_contents _ _ _ _ _ _ H0).
+  rewrite (storebytes_mem_contents _ _ _ _ _ _ STORE).
   rewrite ! PMap.gsspec. destruct (peq b0 b1). subst b0.
   (* block = b1, block = b2 *)
   assert (b3 = b2) by congruence. subst b3.
@@ -2891,9 +3073,9 @@ Proof.
 Qed.
 
 Lemma storebytes_unmapped_inj:
-  forall f m1 b1 ofs bytes1 n1 m2,
+  forall f m1 b1 ofs bytes1 cp n1 m2,
   mem_inj f m1 m2 ->
-  storebytes m1 b1 ofs bytes1 = Some n1 ->
+  storebytes m1 b1 ofs bytes1 cp = Some n1 ->
   f b1 = None ->
   mem_inj f n1 m2.
 Proof.
@@ -2901,34 +3083,40 @@ Proof.
   constructor.
 (* perm *)
   intros. eapply mi_perm0; eauto. eapply perm_storebytes_2; eauto.
+(* own *)
+  intros.
+  eapply mi_own0; try eassumption.
+  eapply storebytes_own_block_inj_2; eassumption.
 (* align *)
   intros. eapply mi_align with (ofs := ofs0) (p := p); eauto.
   red; intros. eapply perm_storebytes_2; eauto.
 (* mem_contents *)
   intros.
-  rewrite (storebytes_mem_contents _ _ _ _ _ H0).
+  rewrite (storebytes_mem_contents _ _ _ _ _ _ H0).
   rewrite PMap.gso. eapply mi_memval0; eauto. eapply perm_storebytes_2; eauto.
   congruence.
 Qed.
 
 Lemma storebytes_outside_inj:
-  forall f m1 m2 b ofs bytes2 m2',
+  forall f m1 m2 b ofs bytes2 cp m2',
   mem_inj f m1 m2 ->
   (forall b' delta ofs',
     f b' = Some(b, delta) ->
     perm m1 b' ofs' Cur Readable ->
     ofs <= ofs' + delta < ofs + Z.of_nat (length bytes2) -> False) ->
-  storebytes m2 b ofs bytes2 = Some m2' ->
+  storebytes m2 b ofs bytes2 cp = Some m2' ->
   mem_inj f m1 m2'.
 Proof.
   intros. inversion H. constructor.
 (* perm *)
   intros. eapply perm_storebytes_1; eauto with mem.
+(* own *)
+  intros. eapply storebytes_own_block_inj_1; eauto.
 (* align *)
   eauto.
 (* mem_contents *)
   intros.
-  rewrite (storebytes_mem_contents _ _ _ _ _ H1).
+  rewrite (storebytes_mem_contents _ _ _ _ _ _ H1).
   rewrite PMap.gsspec. destruct (peq b2 b). subst b2.
   rewrite setN_outside. auto.
   destruct (zlt (ofs0 + delta) ofs); auto.
@@ -2938,10 +3126,10 @@ Proof.
 Qed.
 
 Lemma storebytes_empty_inj:
-  forall f m1 b1 ofs1 m1' m2 b2 ofs2 m2',
+  forall f m1 b1 ofs1 cp1 m1' m2 b2 ofs2 cp2 m2',
   mem_inj f m1 m2 ->
-  storebytes m1 b1 ofs1 nil = Some m1' ->
-  storebytes m2 b2 ofs2 nil = Some m2' ->
+  storebytes m1 b1 ofs1 nil cp1 = Some m1' ->
+  storebytes m2 b2 ofs2 nil cp2 = Some m2' ->
   mem_inj f m1' m2'.
 Proof.
   intros. destruct H. constructor.
@@ -2950,14 +3138,19 @@ Proof.
   eapply perm_storebytes_1; eauto.
   eapply mi_perm0; eauto.
   eapply perm_storebytes_2; eauto.
+(* own *)
+  intros.
+  eapply storebytes_own_block_inj_1; eauto.
+  eapply mi_own0; eauto.
+  eapply storebytes_own_block_inj_2; eauto.
 (* align *)
   intros. eapply mi_align0 with (ofs := ofs) (p := p); eauto.
   red; intros. eapply perm_storebytes_2; eauto.
 (* mem_contents *)
   intros.
   assert (perm m1 b0 ofs Cur Readable). eapply perm_storebytes_2; eauto.
-  rewrite (storebytes_mem_contents _ _ _ _ _ H0).
-  rewrite (storebytes_mem_contents _ _ _ _ _ H1).
+  rewrite (storebytes_mem_contents _ _ _ _ _ _ H0).
+  rewrite (storebytes_mem_contents _ _ _ _ _ _ H1).
   simpl. rewrite ! PMap.gsspec.
   destruct (peq b0 b1); destruct (peq b3 b2); subst; eapply mi_memval0; eauto.
 Qed.
@@ -2974,6 +3167,8 @@ Proof.
   inversion H. constructor.
 (* perm *)
   intros. eapply perm_alloc_1; eauto.
+(* own *)
+  intros. eapply alloc_own_block_other_inj_1; eauto.
 (* align *)
   eauto.
 (* mem_contents *)
@@ -2983,6 +3178,13 @@ Proof.
   assert (valid_block m2 b0) by eauto with mem.
   rewrite <- MEM; simpl. rewrite PMap.gso. eauto with mem.
   rewrite NEXT. eauto with mem.
+Qed.
+
+(* RB: NOTE: Move up, use in previous proofs. *)
+Remark own_block_component :
+  forall m b cp cp', own_block m b cp -> own_block m b cp' -> cp = cp'.
+Proof.
+  congruence.
 Qed.
 
 Lemma alloc_left_unmapped_inj:
@@ -2996,6 +3198,10 @@ Proof.
 (* perm *)
   intros. exploit perm_alloc_inv; eauto. intros.
   destruct (eq_block b0 b1). congruence. eauto.
+(* own *)
+  intros. eapply mi_own0; try eassumption. destruct (eq_block b0 b1).
+  subst b0. congruence.
+  eapply alloc_own_block_other_inj_2; eassumption.
 (* align *)
   intros. eapply mi_align0 with (ofs := ofs) (p := p); eauto.
   red; intros. exploit perm_alloc_inv; eauto.
@@ -3011,6 +3217,7 @@ Qed.
 Definition inj_offset_aligned (delta: Z) (size: Z) : Prop :=
   forall chunk, size_chunk chunk <= size -> (align_chunk chunk | delta).
 
+(* RB: NOTE: Keep track of added assumption and its effect on proofs. *)
 Lemma alloc_left_mapped_inj:
   forall f m1 m2 c lo hi m1' b1 b2 delta,
   mem_inj f m1 m2 ->
@@ -3019,6 +3226,7 @@ Lemma alloc_left_mapped_inj:
   inj_offset_aligned delta (hi-lo) ->
   (forall ofs k p, lo <= ofs < hi -> perm m2 b2 (ofs + delta) k p) ->
   f b1 = Some(b2, delta) ->
+  forall OWN : own_block m2 b2 c,
   mem_inj f m1' m2.
 Proof.
   intros. inversion H. constructor.
@@ -3026,6 +3234,17 @@ Proof.
   intros.
   exploit perm_alloc_inv; eauto. intros. destruct (eq_block b0 b1). subst b0.
   rewrite H4 in H5; inv H5. eauto. eauto.
+(* own *)
+  intros. destruct (eq_block b0 b1).
+  {
+    subst b0. rewrite H4 in H5. inv H5.
+    apply owned_new_block in H0.
+    unfold own_block in *. rewrite H0 in H6. inv H6.
+    exact OWN.
+  }
+  {
+    eapply mi_own0; eauto. eapply alloc_own_block_other_inj_2; eassumption.
+  }
 (* align *)
   intros. destruct (eq_block b0 b1).
   subst b0. assert (delta0 = delta) by congruence. subst delta0.
@@ -3045,14 +3264,16 @@ Proof.
 Qed.
 
 Lemma free_left_inj:
-  forall f m1 m2 b lo hi m1',
+  forall f m1 m2 b lo hi cp m1',
   mem_inj f m1 m2 ->
-  free m1 b lo hi = Some m1' ->
+  free m1 b lo hi cp = Some m1' ->
   mem_inj f m1' m2.
 Proof.
   intros. exploit free_result; eauto. intro FREE. inversion H. constructor.
 (* perm *)
   intros. eauto with mem.
+(* own *)
+  intros. eapply mi_own0; eauto. eapply free_own_block_inj_2; eassumption.
 (* align *)
   intros. eapply mi_align0 with (ofs := ofs) (p := p); eauto.
   red; intros; eapply perm_free_3; eauto.
@@ -3061,9 +3282,9 @@ Proof.
 Qed.
 
 Lemma free_right_inj:
-  forall f m1 m2 b lo hi m2',
+  forall f m1 m2 b lo hi cp m2',
   mem_inj f m1 m2 ->
-  free m2 b lo hi = Some m2' ->
+  free m2 b lo hi cp = Some m2' ->
   (forall b' delta ofs k p,
     f b' = Some(b, delta) ->
     perm m1 b' ofs k p -> lo <= ofs + delta < hi -> False) ->
@@ -3082,6 +3303,8 @@ Proof.
   constructor.
 (* perm *)
   auto.
+(* own *)
+  intros. eapply free_own_block_inj_1; eauto.
 (* align *)
   eapply mi_align0; eauto.
 (* mem_contents *)
@@ -3091,15 +3314,17 @@ Qed.
 (** Preservation of [drop_perm] operations. *)
 
 Lemma drop_unmapped_inj:
-  forall f m1 m2 b lo hi p m1',
+  forall f m1 m2 b lo hi p cp m1',
   mem_inj f m1 m2 ->
-  drop_perm m1 b lo hi p = Some m1' ->
+  drop_perm m1 b lo hi p cp = Some m1' ->
   f b = None ->
   mem_inj f m1' m2.
 Proof.
   intros. inv H. constructor.
 (* perm *)
   intros. eapply mi_perm0; eauto. eapply perm_drop_4; eauto.
+(* own *)
+  intros. eapply mi_own0; eauto. eapply own_block_drop_2; eauto.
 (* align *)
   intros. eapply mi_align0 with (ofs := ofs) (p := p0); eauto.
   red; intros; eapply perm_drop_4; eauto.
@@ -3107,24 +3332,38 @@ Proof.
   intros.
   replace (ZMap.get ofs m1'.(mem_contents)#b1) with (ZMap.get ofs m1.(mem_contents)#b1).
   apply mi_memval0; auto. eapply perm_drop_4; eauto.
-  unfold drop_perm in H0; destruct (range_perm_dec m1 b lo hi Cur Freeable); inv H0; auto.
+  unfold drop_perm in H0;
+  destruct (range_perm_dec m1 b lo hi Cur Freeable);
+  destruct (own_block_dec m1 b cp);
+  inv H0; auto.
 Qed.
 
+(* Definition meminj_no_dispute (f: meminj) (m: mem) : Prop := *)
+(*   forall b1 b1' delta1 cp1 b2 b2' delta2 cp2, *)
+(*   b1 <> b2 -> *)
+(*   f b1 = Some (b1', delta1) -> *)
+(*   f b2 = Some (b2', delta2) -> *)
+(*   own_block m b1 cp1 -> *)
+(*   own_block m b2 cp2 -> *)
+(*   b1' <> b2' \/ cp1 <> cp2. *)
+
 Lemma drop_mapped_inj:
-  forall f m1 m2 b1 b2 delta lo hi p m1',
+  forall f m1 m2 b1 b2 delta lo hi p cp m1',
   mem_inj f m1 m2 ->
-  drop_perm m1 b1 lo hi p = Some m1' ->
+  drop_perm m1 b1 lo hi p cp = Some m1' ->
   meminj_no_overlap f m1 ->
+  (* forall DISP : meminj_no_dispute f m1, *)
   f b1 = Some(b2, delta) ->
   exists m2',
-      drop_perm m2 b2 (lo + delta) (hi + delta) p = Some m2'
+      drop_perm m2 b2 (lo + delta) (hi + delta) p cp = Some m2'
    /\ mem_inj f m1' m2'.
 Proof.
   intros.
-  assert ({ m2' | drop_perm m2 b2 (lo + delta) (hi + delta) p = Some m2' }).
+  assert ({ m2' | drop_perm m2 b2 (lo + delta) (hi + delta) p cp = Some m2' }).
   apply range_perm_drop_2. red; intros.
   replace ofs with ((ofs - delta) + delta) by omega.
   eapply perm_inj; eauto. eapply range_perm_drop_1; eauto. omega.
+  eapply mi_own; eauto. eapply own_block_drop_3; eauto.
   destruct X as [m2' DROP]. exists m2'; split; auto.
   inv H.
   constructor.
@@ -3153,6 +3392,12 @@ Proof.
   eapply perm_drop_4; eauto. eapply perm_max. apply perm_implies with p0. eauto.
   eauto with mem.
   intuition.
+(* own *)
+  intros.
+  pose proof own_block_drop_2 _ _ _ _ _ _ _ H0 _ _ H3 as Hown1.
+  pose proof own_block_drop_3 _ _ _ _ _ _ _ DROP as Hown2.
+  pose proof mi_own0 _ _ _ _ H Hown1 as Hown3.
+  eapply own_block_drop_1; eassumption.
 (* align *)
   intros. eapply mi_align0 with (ofs := ofs) (p := p0); eauto.
   red; intros; eapply perm_drop_4; eauto.
@@ -3161,13 +3406,19 @@ Proof.
   replace (m1'.(mem_contents)#b0) with (m1.(mem_contents)#b0).
   replace (m2'.(mem_contents)#b3) with (m2.(mem_contents)#b3).
   apply mi_memval0; auto. eapply perm_drop_4; eauto.
-  unfold drop_perm in DROP; destruct (range_perm_dec m2 b2 (lo + delta) (hi + delta) Cur Freeable); inv DROP; auto.
-  unfold drop_perm in H0; destruct (range_perm_dec m1 b1 lo hi Cur Freeable); inv H0; auto.
+  unfold drop_perm in DROP;
+  destruct (range_perm_dec m2 b2 (lo + delta) (hi + delta) Cur Freeable);
+  destruct (own_block_dec m2 b2 cp);
+  inv DROP; auto.
+  unfold drop_perm in H0;
+  destruct (range_perm_dec m1 b1 lo hi Cur Freeable);
+  destruct (own_block_dec m1 b1 cp);
+  inv H0; auto.
 Qed.
 
-Lemma drop_outside_inj: forall f m1 m2 b lo hi p m2',
+Lemma drop_outside_inj: forall f m1 m2 b lo hi p cp m2',
   mem_inj f m1 m2 ->
-  drop_perm m2 b lo hi p = Some m2' ->
+  drop_perm m2 b lo hi p cp = Some m2' ->
   (forall b' delta ofs' k p,
     f b' = Some(b, delta) ->
     perm m1 b' ofs' k p ->
@@ -3181,13 +3432,18 @@ Proof.
   destruct (zlt (ofs + delta) lo); auto.
   destruct (zle hi (ofs + delta)); auto.
   byContradiction. exploit H1; eauto. omega.
+  (* own *)
+  intros. eapply own_block_drop_1; eauto.
   (* align *)
   eapply mi_align0; eauto.
   (* contents *)
   intros.
   replace (m2'.(mem_contents)#b2) with (m2.(mem_contents)#b2).
   apply mi_memval0; auto.
-  unfold drop_perm in H0; destruct (range_perm_dec m2 b lo hi Cur Freeable); inv H0; auto.
+  unfold drop_perm in H0;
+  destruct (range_perm_dec m2 b lo hi Cur Freeable);
+  destruct (own_block_dec m2 b cp);
+  inv H0; auto.
 Qed.
 
 (** * Memory extensions *)
@@ -3214,6 +3470,7 @@ Theorem extends_refl:
 Proof.
   intros. constructor. auto. constructor.
   intros. unfold inject_id in H; inv H. replace (ofs + 0) with ofs by omega. auto.
+  intros. unfold inject_id in H; inv H. assumption.
   intros. unfold inject_id in H; inv H. apply Z.divide_0_r.
   intros. unfold inject_id in H; inv H. replace (ofs + 0) with ofs by omega.
   apply memval_lessdef_refl.
@@ -3221,10 +3478,10 @@ Proof.
 Qed.
 
 Theorem load_extends:
-  forall chunk m1 m2 b ofs v1,
+  forall chunk m1 m2 b ofs cp v1,
   extends m1 m2 ->
-  load chunk m1 b ofs = Some v1 ->
-  exists v2, load chunk m2 b ofs = Some v2 /\ Val.lessdef v1 v2.
+  load chunk m1 b ofs cp = Some v1 ->
+  exists v2, load chunk m2 b ofs cp = Some v2 /\ Val.lessdef v1 v2.
 Proof.
   intros. inv H. exploit load_inj; eauto. unfold inject_id; reflexivity.
   intros [v2 [A B]]. exists v2; split.
@@ -3233,11 +3490,11 @@ Proof.
 Qed.
 
 Theorem loadv_extends:
-  forall chunk m1 m2 addr1 addr2 v1,
+  forall chunk m1 m2 addr1 cp addr2 v1,
   extends m1 m2 ->
-  loadv chunk m1 addr1 = Some v1 ->
+  loadv chunk m1 addr1 cp = Some v1 ->
   Val.lessdef addr1 addr2 ->
-  exists v2, loadv chunk m2 addr2 = Some v2 /\ Val.lessdef v1 v2.
+  exists v2, loadv chunk m2 addr2 cp = Some v2 /\ Val.lessdef v1 v2.
 Proof.
   unfold loadv; intros. inv H1.
   destruct addr2; try congruence. eapply load_extends; eauto.
@@ -3245,10 +3502,10 @@ Proof.
 Qed.
 
 Theorem loadbytes_extends:
-  forall m1 m2 b ofs len bytes1,
+  forall m1 m2 b ofs len cp bytes1,
   extends m1 m2 ->
-  loadbytes m1 b ofs len = Some bytes1 ->
-  exists bytes2, loadbytes m2 b ofs len = Some bytes2
+  loadbytes m1 b ofs len cp = Some bytes1 ->
+  exists bytes2, loadbytes m2 b ofs len cp = Some bytes2
               /\ list_forall2 memval_lessdef bytes1 bytes2.
 Proof.
   intros. inv H.
@@ -3256,12 +3513,12 @@ Proof.
 Qed.
 
 Theorem store_within_extends:
-  forall chunk m1 m2 b ofs v1 m1' v2,
+  forall chunk m1 m2 b ofs v1 cp m1' v2,
   extends m1 m2 ->
-  store chunk m1 b ofs v1 = Some m1' ->
+  store chunk m1 b ofs v1 cp = Some m1' ->
   Val.lessdef v1 v2 ->
   exists m2',
-     store chunk m2 b ofs v2 = Some m2'
+     store chunk m2 b ofs v2 cp = Some m2'
   /\ extends m1' m2'.
 Proof.
   intros. inversion H.
@@ -3273,34 +3530,34 @@ Proof.
   exists m2'; split.
   replace (ofs + 0) with ofs in A by omega. auto.
   constructor; auto.
-  rewrite (nextblock_store _ _ _ _ _ _ H0).
-  rewrite (nextblock_store _ _ _ _ _ _ A).
+  rewrite (nextblock_store _ _ _ _ _ _ _ H0).
+  rewrite (nextblock_store _ _ _ _ _ _ _ A).
   auto.
   intros. exploit mext_perm_inv0; intuition eauto using perm_store_1, perm_store_2.
 Qed.
 
 Theorem store_outside_extends:
-  forall chunk m1 m2 b ofs v m2',
+  forall chunk m1 m2 b ofs v cp m2',
   extends m1 m2 ->
-  store chunk m2 b ofs v = Some m2' ->
+  store chunk m2 b ofs v cp = Some m2' ->
   (forall ofs', perm m1 b ofs' Cur Readable -> ofs <= ofs' < ofs + size_chunk chunk -> False) ->
   extends m1 m2'.
 Proof.
   intros. inversion H. constructor.
-  rewrite (nextblock_store _ _ _ _ _ _ H0). auto.
+  rewrite (nextblock_store _ _ _ _ _ _ _ H0). auto.
   eapply store_outside_inj; eauto.
   unfold inject_id; intros. inv H2. eapply H1; eauto. omega.
   intros. eauto using perm_store_2.
 Qed.
 
 Theorem storev_extends:
-  forall chunk m1 m2 addr1 v1 m1' addr2 v2,
+  forall chunk m1 m2 addr1 v1 cp m1' addr2 v2,
   extends m1 m2 ->
-  storev chunk m1 addr1 v1 = Some m1' ->
+  storev chunk m1 addr1 v1 cp = Some m1' ->
   Val.lessdef addr1 addr2 ->
   Val.lessdef v1 v2 ->
   exists m2',
-     storev chunk m2 addr2 v2 = Some m2'
+     storev chunk m2 addr2 v2 cp = Some m2'
   /\ extends m1' m2'.
 Proof.
   unfold storev; intros. inv H1.
@@ -3309,12 +3566,12 @@ Proof.
 Qed.
 
 Theorem storebytes_within_extends:
-  forall m1 m2 b ofs bytes1 m1' bytes2,
+  forall m1 m2 b ofs bytes1 cp m1' bytes2,
   extends m1 m2 ->
-  storebytes m1 b ofs bytes1 = Some m1' ->
+  storebytes m1 b ofs bytes1 cp = Some m1' ->
   list_forall2 memval_lessdef bytes1 bytes2 ->
   exists m2',
-     storebytes m2 b ofs bytes2 = Some m2'
+     storebytes m2 b ofs bytes2 cp = Some m2'
   /\ extends m1' m2'.
 Proof.
   intros. inversion H.
@@ -3325,21 +3582,21 @@ Proof.
   exists m2'; split.
   replace (ofs + 0) with ofs in A by omega. auto.
   constructor; auto.
-  rewrite (nextblock_storebytes _ _ _ _ _ H0).
-  rewrite (nextblock_storebytes _ _ _ _ _ A).
+  rewrite (nextblock_storebytes _ _ _ _ _ _ H0).
+  rewrite (nextblock_storebytes _ _ _ _ _ _ A).
   auto.
   intros. exploit mext_perm_inv0; intuition eauto using perm_storebytes_1, perm_storebytes_2.
 Qed.
 
 Theorem storebytes_outside_extends:
-  forall m1 m2 b ofs bytes2 m2',
+  forall m1 m2 b ofs bytes2 cp m2',
   extends m1 m2 ->
-  storebytes m2 b ofs bytes2 = Some m2' ->
+  storebytes m2 b ofs bytes2 cp = Some m2' ->
   (forall ofs', perm m1 b ofs' Cur Readable -> ofs <= ofs' < ofs + Z.of_nat (length bytes2) -> False) ->
   extends m1 m2'.
 Proof.
   intros. inversion H. constructor.
-  rewrite (nextblock_storebytes _ _ _ _ _ H0). auto.
+  rewrite (nextblock_storebytes _ _ _ _ _ _ H0). auto.
   eapply storebytes_outside_inj; eauto.
   unfold inject_id; intros. inv H2. eapply H1; eauto. omega.
   intros. eauto using perm_storebytes_2.
@@ -3374,6 +3631,7 @@ Proof.
   eapply perm_implies with Freeable; auto with mem.
   eapply perm_alloc_2; eauto.
   omega.
+  eapply owned_new_block; eassumption.
   intros. eapply perm_alloc_inv in H; eauto.
   generalize (perm_alloc_inv _ _ _ _ _ _ H0 b0 ofs Max Nonempty); intros PERM.
   destruct (eq_block b0 b).
@@ -3386,13 +3644,13 @@ Proof.
 Qed.
 
 Theorem free_left_extends:
-  forall m1 m2 b lo hi m1',
+  forall m1 m2 b lo hi cp m1',
   extends m1 m2 ->
-  free m1 b lo hi = Some m1' ->
+  free m1 b lo hi cp = Some m1' ->
   extends m1' m2.
 Proof.
   intros. inv H. constructor.
-  rewrite (nextblock_free _ _ _ _ _ H0). auto.
+  rewrite (nextblock_free _ _ _ _ _ _ H0). auto.
   eapply free_left_inj; eauto.
   intros. exploit mext_perm_inv0; eauto. intros [A|A].
   eapply perm_free_inv in A; eauto. destruct A as [[A B]|A]; auto.
@@ -3401,37 +3659,41 @@ Proof.
 Qed.
 
 Theorem free_right_extends:
-  forall m1 m2 b lo hi m2',
+  forall m1 m2 b lo hi cp m2',
   extends m1 m2 ->
-  free m2 b lo hi = Some m2' ->
+  free m2 b lo hi cp = Some m2' ->
   (forall ofs k p, perm m1 b ofs k p -> lo <= ofs < hi -> False) ->
   extends m1 m2'.
 Proof.
   intros. inv H. constructor.
-  rewrite (nextblock_free _ _ _ _ _ H0). auto.
+  rewrite (nextblock_free _ _ _ _ _ _ H0). auto.
   eapply free_right_inj; eauto.
   unfold inject_id; intros. inv H. eapply H1; eauto. omega.
   intros. eauto using perm_free_3.
 Qed.
 
 Theorem free_parallel_extends:
-  forall m1 m2 b lo hi m1',
+  forall m1 m2 b lo hi cp m1',
   extends m1 m2 ->
-  free m1 b lo hi = Some m1' ->
+  free m1 b lo hi cp = Some m1' ->
   exists m2',
-     free m2 b lo hi = Some m2'
+     free m2 b lo hi cp = Some m2'
   /\ extends m1' m2'.
 Proof.
   intros. inversion H.
-  assert ({ m2': mem | free m2 b lo hi = Some m2' }).
+  assert ({ m2': mem | free m2 b lo hi cp = Some m2' }).
     apply range_perm_free. red; intros.
     replace ofs with (ofs + 0) by omega.
     eapply perm_inj with (b1 := b); eauto.
     eapply free_range_perm; eauto.
+    (* own *)
+    unfold inject_id in mext_inj0; inv mext_inj0.
+    eapply mi_own0; eauto.
+    eapply free_own_block_1; eassumption.
   destruct X as [m2' FREE]. exists m2'; split; auto.
   constructor.
-  rewrite (nextblock_free _ _ _ _ _ H0).
-  rewrite (nextblock_free _ _ _ _ _ FREE). auto.
+  rewrite (nextblock_free _ _ _ _ _ _ H0).
+  rewrite (nextblock_free _ _ _ _ _ _ FREE). auto.
   eapply free_right_inj with (m1 := m1'); eauto.
   eapply free_left_inj; eauto.
   unfold inject_id; intros. inv H1.
@@ -3466,8 +3728,8 @@ Proof.
 Qed.
 
 Theorem valid_access_extends:
-  forall m1 m2 chunk b ofs p,
-  extends m1 m2 -> valid_access m1 chunk b ofs p -> valid_access m2 chunk b ofs p.
+  forall m1 m2 chunk b ofs p cp,
+  extends m1 m2 -> valid_access m1 chunk b ofs p cp -> valid_access m2 chunk b ofs p cp.
 Proof.
   intros. inv H. replace ofs with (ofs + 0) by omega.
   eapply valid_access_inj; eauto. auto.
